Porting framed derivatives to HS_Lens_ODEs

HS_Lens_ODEs.thy
@@ -8,7 +8,7 @@ cleaner presentation. \<close>
 theory HS_Lens_ODEs
   imports 
     "HS_ODEs" 
-    "Hybrid-Library.Cont_Lens" 
+    "Hybrid-Library.Cont_Lens"
     "Shallow-Expressions.Shallow_Expressions"
 begin
 
@@ -21,56 +21,63 @@ lenses @{term "x :: 'c \<Longrightarrow> 's"}, we lift entities from @{typ 'c} t
 no_notation id_lens ("1\<^sub>L")
 notation id_lens ("\<one>\<^sub>L")
 
-subsection \<open> Framing  \<close>
+subsection \<open> Framing and lifting \<close>
 
 definition lframe_fun :: "('c \<Longrightarrow> 's) \<Rightarrow> ('s \<Rightarrow> 'v) \<Rightarrow> 's \<Rightarrow> ('c \<Rightarrow> 'v)" (infixr "\<down>\<^sub>F\<index>" 100)
   where "(F\<down>\<^sub>F\<^bsub>x\<^esub> s) c = F (put\<^bsub>x\<^esub> s c)"
 
-definition llift_fun :: "('c \<Longrightarrow> 's) \<Rightarrow> ('c \<Rightarrow> 'v) \<Rightarrow> ('s \<Rightarrow> 'v)" (infixr "\<up>\<^sub>F\<index>" 100)
-  where "F\<up>\<^sub>F\<^bsub>x\<^esub> s \<equiv>  F (get\<^bsub>x\<^esub> s)"
+lemma lframe_fun_alt [expr_defs]: "(F\<down>\<^sub>F\<^bsub>x\<^esub> s) = (\<lambda>c. F (put\<^bsub>x\<^esub> s c))"
+  by (auto simp: lframe_fun_def)
 
-definition llift_set :: "('c \<Longrightarrow> 's) \<Rightarrow> 'c set \<Rightarrow> 's \<Rightarrow> 's set" (infixr "\<up>\<^sub>S\<^sub>e\<^sub>t\<index>" 100)
-  where "X\<up>\<^sub>S\<^sub>e\<^sub>t\<^bsub>x\<^esub> s \<equiv>  \<P> (\<lambda>c. put\<^bsub>x\<^esub> s c) X"
+definition llift_fun :: "('c \<Longrightarrow> 's) \<Rightarrow> ('c \<Rightarrow> 'v) \<Rightarrow> ('s \<Rightarrow> 'v)" (infixr "\<up>\<^sub>F\<index>" 100)
+  where [expr_defs]: "F\<up>\<^sub>F\<^bsub>x\<^esub> s \<equiv>  F (get\<^bsub>x\<^esub> s)"
 
 definition lframe_set :: "('c \<Longrightarrow> 's) \<Rightarrow> 's set \<Rightarrow> 'c set" ("_\<down>\<^sub>S\<^sub>e\<^sub>t\<index>" [100] 100)
-  where "X\<down>\<^sub>S\<^sub>e\<^sub>t\<^bsub>x\<^esub> = \<P> get\<^bsub>x\<^esub> X"
+  where [expr_defs]: "X\<down>\<^sub>S\<^sub>e\<^sub>t\<^bsub>x\<^esub> = \<P> get\<^bsub>x\<^esub> X"
+
+definition llift_set :: "('c \<Longrightarrow> 's) \<Rightarrow> 'c set \<Rightarrow> 's \<Rightarrow> 's set" (infixr "\<up>\<^sub>S\<^sub>e\<^sub>t\<index>" 100)
+  where [expr_defs]: "X\<up>\<^sub>S\<^sub>e\<^sub>t\<^bsub>x\<^esub> s \<equiv> \<P> (\<lambda>c. put\<^bsub>x\<^esub> s c) X"
 
 definition lframe_pred :: "('c \<Longrightarrow> 's) \<Rightarrow> ('s \<Rightarrow> bool) \<Rightarrow> ('c \<Rightarrow> bool)" ("_\<down>\<^sub>P\<index>" [100] 1000)
-  where "P\<down>\<^sub>P\<^bsub>x\<^esub> c \<longleftrightarrow> c \<in> {s. P s}\<down>\<^sub>S\<^sub>e\<^sub>t\<^bsub>x\<^esub>"
+  where [expr_defs]: "P\<down>\<^sub>P\<^bsub>x\<^esub> c \<longleftrightarrow> c \<in> {s. P s}\<down>\<^sub>S\<^sub>e\<^sub>t\<^bsub>x\<^esub>"
 
 lemma lframe_pred_iff_pred_as_fun: 
   "vwb_lens x \<Longrightarrow> P\<down>\<^sub>P\<^bsub>x\<^esub> c \<longleftrightarrow> (\<exists>s. (P\<down>\<^sub>F\<^bsub>x\<^esub> s) c)"
-  unfolding lframe_pred_def lframe_fun_def lframe_set_def
   by (expr_auto add: image_iff)
     (metis vwb_lens_def wb_lens.get_put)
 
 lemma lframe_set_Collect_llift_fun: 
   "vwb_lens x \<Longrightarrow> \<P> get\<^bsub>x\<^esub> UNIV = UNIV \<Longrightarrow> {s. P\<up>\<^sub>F\<^bsub>x\<^esub> s}\<down>\<^sub>S\<^sub>e\<^sub>t\<^bsub>x\<^esub> = {c. P c}"
-  by (auto simp: llift_fun_def lframe_set_def)
+  by expr_auto
 
 lemma llift_set_Collect_lframe_pred: 
   "vwb_lens x \<Longrightarrow> {c. P\<down>\<^sub>P\<^bsub>x\<^esub> c}\<up>\<^sub>S\<^sub>e\<^sub>t\<^bsub>x\<^esub> s = {put\<^bsub>x\<^esub> s (get\<^bsub>x\<^esub> s') |s'. P s'}"
-  by (auto simp: lframe_pred_def llift_set_def image_iff lframe_set_def)
+  by expr_auto
 
 lemma Un_llift_set_lframe_pred_supset: 
   "vwb_lens x \<Longrightarrow> {s. P s} \<subseteq> (\<Union>s. {c. P\<down>\<^sub>P\<^bsub>x\<^esub> c}\<up>\<^sub>S\<^sub>e\<^sub>t\<^bsub>x\<^esub> s)"
   by (auto simp: lframe_pred_def llift_set_def image_iff lframe_set_def)
     (metis vwb_lens.put_eq)
 
-
-subsection \<open> Framed orbitals  \<close>
-
 text \<open> Localise a substitution using a lens. Useful for localising both ODEs and flows. \<close>
 
-definition lframe_tsubst :: "('c \<Longrightarrow> 's) \<Rightarrow> ('t \<Rightarrow> 's \<Rightarrow> 's) \<Rightarrow> 's \<Rightarrow> ('t \<Rightarrow> 'c \<Rightarrow> 'c)"
-  where "lframe_tsubst x F s t c \<equiv> get\<^bsub>x\<^esub> ((F t \<down>\<^sub>F\<^bsub>x\<^esub> s) c)"
+definition lframe_subst :: "('c \<Longrightarrow> 's) \<Rightarrow> ('s \<Rightarrow> 's) \<Rightarrow> 's \<Rightarrow> ('c \<Rightarrow> 'c)" (infixr "\<down>\<^sub>S\<^sub>u\<^sub>b\<^sub>s\<^sub>t\<index>" 100)
+  where "(\<sigma>\<down>\<^sub>S\<^sub>u\<^sub>b\<^sub>s\<^sub>t\<^bsub>x\<^esub> s) c \<equiv> get\<^bsub>x\<^esub> ((\<sigma> \<down>\<^sub>F\<^bsub>x\<^esub> s) c)"
+
+lemma lframe_subst_alt [expr_defs]: 
+  "(\<down>\<^sub>S\<^sub>u\<^sub>b\<^sub>s\<^sub>t\<^bsub>x\<^esub>) \<sigma> \<equiv> (\<lambda>s c. get\<^bsub>x\<^esub> (\<sigma> (put\<^bsub>x\<^esub> s c)))"
+  unfolding lframe_subst_def
+  by expr_simp
 
 abbreviation tsubst2vecf :: "('c::real_normed_vector \<Longrightarrow> 's) 
   \<Rightarrow> (real \<Rightarrow> 's \<Rightarrow> 's) \<Rightarrow> 's \<Rightarrow> real \<Rightarrow> 'c \<Rightarrow> 'c" (infixr "\<down>\<^sub>V\<^sub>e\<^sub>c\<index>" 100)
-  where "(F\<down>\<^sub>V\<^sub>e\<^sub>c\<^bsub>x\<^esub> s) t c \<equiv> lframe_tsubst x F s t c"
+  where "(F\<down>\<^sub>V\<^sub>e\<^sub>c\<^bsub>x\<^esub> s) t c \<equiv> (F t \<down>\<^sub>S\<^sub>u\<^sub>b\<^sub>s\<^sub>t\<^bsub>x\<^esub> s) c"
 
-lemma tsubst2vecf_eq[expr_defs]: "F \<down>\<^sub>V\<^sub>e\<^sub>c\<^bsub>x\<^esub> s = (\<lambda> t c. get\<^bsub>x\<^esub> (F t (put\<^bsub>x\<^esub> s c)))"
-  by (auto simp: lframe_tsubst_def fun_eq_iff lframe_fun_def)
+lemma tsubst2vecf_eq: "F\<down>\<^sub>V\<^sub>e\<^sub>c\<^bsub>x\<^esub> s = (\<lambda> t c. get\<^bsub>x\<^esub> (F t (put\<^bsub>x\<^esub> s c)))"
+  by (auto simp: lframe_subst_def fun_eq_iff lframe_fun_def)
+
+
+subsection \<open> Framed orbitals  \<close>
 
 text \<open> A version of orbital localised by a lens \<close>
 
@@ -96,7 +103,7 @@ lemma g_orbital_onI:
   using assms unfolding g_orbital_on_eq tsubst2vecf_eq by auto
 
 
-subsection \<open> Framed differential dnvariants \<close>
+subsection \<open> Framed differential invariants \<close>
 
 definition diff_inv_on :: "('c:: real_normed_vector \<Longrightarrow> 'a) \<Rightarrow> (real \<Rightarrow> 'a \<Rightarrow> 'a) 
   \<Rightarrow> ('a \<Rightarrow> bool) \<Rightarrow> ('c \<Rightarrow> real set) \<Rightarrow> 'c set \<Rightarrow> real \<Rightarrow> ('a \<Rightarrow> bool) \<Rightarrow> bool" 
@@ -129,7 +136,382 @@ next
 qed
 
 
-subsubsection \<open> framed differential invariant rules \<close>
+subsection \<open> framed differentiation \<close>
+
+lemma has_derivative_discr_expr:
+  "\<lbrakk>vwb_lens x; $x \<sharp> (expr)\<^sub>e\<rbrakk> \<Longrightarrow> ((\<lambda>c. expr (put\<^bsub>x\<^esub> s c)) has_derivative (\<lambda>c. 0)) (at (get\<^bsub>x\<^esub> s) within S)"
+  by expr_auto
+
+definition ldifferentiable_expr :: "('c::real_normed_vector \<Longrightarrow> 's) \<Rightarrow> 'c set
+  \<Rightarrow> ('s \<Rightarrow> 'v::real_normed_vector) \<Rightarrow> bool"
+  where [expr_defs]: "ldifferentiable_expr x S expr 
+  \<longleftrightarrow> (\<forall>s. (\<lambda>c. expr (put\<^bsub>x\<^esub> s c)) differentiable (at (get\<^bsub>x\<^esub> s) within S))"
+
+syntax 
+  "_differentiable_expr_on" :: "logic \<Rightarrow> logic \<Rightarrow> logic \<Rightarrow> logic" ("differentiable\<index> _ on _" [0,100] 100)
+  "_differentiable_expr" :: "logic \<Rightarrow> logic \<Rightarrow> logic" ("differentiable\<index> _ " [100] 100)
+
+translations 
+  "differentiable\<^bsub>x\<^esub> expr on S" == "CONST ldifferentiable_expr x S (expr)\<^sub>e"
+  "differentiable\<^bsub>x\<^esub> expr" == "CONST ldifferentiable_expr x (CONST UNIV) (expr)\<^sub>e"
+
+named_theorems ldifferentiable
+
+lemma differentiable_number [ldifferentiable]:
+  "differentiable\<^bsub>x\<^esub> 0 on S" 
+  "differentiable\<^bsub>x\<^esub> 1 on S" 
+  "differentiable\<^bsub>x\<^esub> (numeral \<guillemotleft>n\<guillemotright>) on S"
+  by (simp_all add: expr_defs)
+
+lemma differentiable_const [ldifferentiable]:
+  "differentiable\<^bsub>x\<^esub> \<guillemotleft>k\<guillemotright> on S"
+  by (simp_all add: expr_defs)
+
+lemma differentiable_discr_expr [ldifferentiable]:
+  "\<lbrakk> vwb_lens x; $x \<sharp> (expr)\<^sub>e \<rbrakk> \<Longrightarrow> differentiable\<^bsub>x\<^esub> expr on S"
+  using differentiable_def has_derivative_discr_expr
+  by (fastforce simp add: ldifferentiable_expr_def)
+
+lemma differentiable_plus [ldifferentiable]:
+  assumes "differentiable\<^bsub>x\<^esub> expr1 on S" "differentiable\<^bsub>x\<^esub> expr2 on S"
+  shows "differentiable\<^bsub>x\<^esub> (expr1 + expr2) on S"
+  using assms by (simp add: expr_defs)
+
+lemma differentiable_minus [ldifferentiable]:
+  assumes "differentiable\<^bsub>x\<^esub> expr1 on S" "differentiable\<^bsub>x\<^esub> expr2 on S"
+  shows "differentiable\<^bsub>x\<^esub> (expr1 - expr2) on S"
+  using assms by (simp add: expr_defs)
+
+lemma differentiable_times [ldifferentiable]:
+  fixes expr1 expr2 :: "'s \<Rightarrow> 'v::real_normed_field"
+  assumes "differentiable\<^bsub>x\<^esub> expr1 on S" "differentiable\<^bsub>x\<^esub> expr2 on S"
+  shows "differentiable\<^bsub>x\<^esub> (expr1 * expr2) on S"
+  using assms by (simp add: expr_defs)
+
+lemma differentiable_inverse [ldifferentiable]:
+  fixes expr :: "'s \<Rightarrow> 'v::real_normed_field"
+  assumes "`expr \<noteq> 0`" "differentiable\<^bsub>x\<^esub> expr on S"
+  shows "differentiable\<^bsub>x\<^esub> (inverse expr) on S"
+  using assms by (auto simp add: expr_defs)
+
+lemma differentiable_divide [ldifferentiable]:
+  fixes expr1 expr2 :: "'s \<Rightarrow> 'v::real_normed_field"
+  assumes "`expr2 \<noteq> 0`" "differentiable\<^bsub>x\<^esub> expr1 on S" "differentiable\<^bsub>x\<^esub> expr2 on S"
+  shows "differentiable\<^bsub>x\<^esub> (expr1 / expr2) on S"
+  using assms by (auto simp add: expr_defs)
+
+lemma differentiable_inner [ldifferentiable]:
+  assumes "differentiable\<^bsub>x\<^esub> expr1 on S" "differentiable\<^bsub>x\<^esub> expr2 on S"
+  shows "differentiable\<^bsub>x\<^esub> (expr1 \<bullet> expr2) on S"
+  using assms by (simp add: expr_defs)
+
+lemma differentiable_scaleR [ldifferentiable]:
+  assumes "differentiable\<^bsub>x\<^esub> r on S" "differentiable\<^bsub>x\<^esub> expr on S"
+  shows "differentiable\<^bsub>x\<^esub> (r *\<^sub>R expr) on S"
+  using assms by (simp add: expr_defs)
+
+lemma differentiable_power [ldifferentiable]:
+  fixes expr :: "'s \<Rightarrow> 'v::real_normed_field"
+  assumes "differentiable\<^bsub>x\<^esub> expr on S"
+  shows "differentiable\<^bsub>x\<^esub> (expr^\<guillemotleft>n\<guillemotright>) on S"
+  using assms by (simp add: expr_defs)
+
+lemma sublens_obs_create: "\<lbrakk> mwb_lens X; Y \<subseteq>\<^sub>L X \<rbrakk> \<Longrightarrow> get\<^bsub>Y\<^esub> (put\<^bsub>X\<^esub> v s) = get\<^bsub>Y\<^esub> (create\<^bsub>X\<^esub> s)"
+  by (simp add: lens_create_def sublens_obs_get)
+
+lemma differentiable_cvar [ldifferentiable]:
+  assumes "vwb_lens X" "x \<subseteq>\<^sub>L X" "bounded_linear (get\<^bsub>x /\<^sub>L X\<^esub>)"
+  shows "differentiable\<^bsub>X\<^esub> $x on S"
+  using assms apply (clarsimp simp add: expr_defs lens_quotient_def sublens_obs_create)
+  using bounded_linear_imp_differentiable by blast
+
+lemma differentiable_dvar [ldifferentiable]:
+  assumes "x \<bowtie> y"
+  shows "differentiable\<^bsub>y\<^esub> $x on S"
+  using assms by (auto simp add: expr_defs)
+
+(* should we generalise and make it "at (get\<^bsub>x\<^esub> s) within S"? It does not seem 
+  necessary for open sets (c.f. thm at_within_open at_within_open_subset at_within_Icc_at). 
+  But what about closed sets (c.f. darboux competition example)? *)
+(* What benefits can we get by making the substitution time-dependent? *)
+definition lframe_frechetD :: "('c::real_normed_vector \<Longrightarrow> 's)
+  \<Rightarrow> ('s \<Rightarrow> 's) \<Rightarrow> ('s \<Rightarrow> 'v::real_normed_vector) \<Rightarrow> 's \<Rightarrow> 'v" 
+  where "lframe_frechetD x \<sigma> expr s = \<partial> (expr\<down>\<^sub>F\<^bsub>x\<^esub> s) (at (get\<^bsub>x\<^esub> s)) (get\<^bsub>x\<^esub> (\<sigma> s))"
+
+lemma lframe_frechetD_alt [expr_defs]: "lframe_frechetD x \<sigma> expr 
+  = (\<lambda>s. frechet_derivative (\<lambda>c. expr (put\<^bsub>x\<^esub> s c)) (at (get\<^bsub>x\<^esub> s)) (get\<^bsub>x\<^esub> (\<sigma> s)))"
+  by (simp add: expr_defs lframe_frechetD_def fun_eq_iff)
+
+expr_ctr lframe_frechetD
+
+syntax
+  "_lframeD"  :: "logic \<Rightarrow> logic \<Rightarrow> logic \<Rightarrow> logic"  ("\<D>\<index>\<langle>_\<rangle> _" [0, 100] 100)
+
+translations
+  "_lframeD x \<sigma> expr" == "CONST lframe_frechetD x \<sigma> (expr)\<^sub>e"
+
+named_theorems framed_derivs
+
+lemma lframeD_zero [framed_derivs]: "\<D>\<^bsub>x\<^esub>\<langle>\<sigma>\<rangle> 0 = (0)\<^sub>e"
+  by (simp add: expr_defs)
+
+lemma lframeD_one [framed_derivs]: "\<D>\<^bsub>x\<^esub>\<langle>\<sigma>\<rangle> 1 = (0)\<^sub>e"
+  by (simp add: expr_defs)
+
+lemma lframeD_numeral [framed_derivs]: "\<D>\<^bsub>x\<^esub>\<langle>\<sigma>\<rangle> numeral \<guillemotleft>n\<guillemotright> = (0)\<^sub>e"
+  by (simp add: expr_defs)
+
+lemma lframeD_const [framed_derivs]: "\<D>\<^bsub>x\<^esub>\<langle>\<sigma>\<rangle> \<guillemotleft>k\<guillemotright> = (0)\<^sub>e"
+  by (simp add: expr_defs)
+
+lemma lframeD_discr_expr [framed_derivs]:
+  "\<lbrakk> vwb_lens x; $x \<sharp> (expr)\<^sub>e \<rbrakk> \<Longrightarrow> \<D>\<^bsub>x\<^esub>\<langle>\<sigma>\<rangle> expr = (0)\<^sub>e"
+  by expr_simp
+
+lemma lframeD_plus [framed_derivs]:
+  "\<lbrakk>differentiable\<^bsub>x\<^esub> expr1 ; differentiable\<^bsub>x\<^esub> expr2\<rbrakk> 
+  \<Longrightarrow> \<D>\<^bsub>x\<^esub>\<langle>\<sigma>\<rangle> (expr1 + expr2) = (\<D>\<^bsub>x\<^esub>\<langle>\<sigma>\<rangle> expr1 + \<D>\<^bsub>x\<^esub>\<langle>\<sigma>\<rangle> expr2)\<^sub>e"
+  by (simp add: expr_defs fun_eq_iff frechet_derivative_plus)
+
+lemma lframeD_minus [framed_derivs]:
+  "\<lbrakk>differentiable\<^bsub>x\<^esub> expr1 ; differentiable\<^bsub>x\<^esub> expr2 \<rbrakk> 
+  \<Longrightarrow> \<D>\<^bsub>x\<^esub>\<langle>\<sigma>\<rangle> (expr1 - expr2) = (\<D>\<^bsub>x\<^esub>\<langle>\<sigma>\<rangle> expr1 - \<D>\<^bsub>x\<^esub>\<langle>\<sigma>\<rangle> expr2)\<^sub>e"
+  by (simp add: expr_defs fun_eq_iff frechet_derivative_minus)
+
+lemma lframeD_times [framed_derivs]:
+  fixes expr1 expr2 :: "'s \<Rightarrow> 'v::real_normed_field"
+  assumes "vwb_lens x" "differentiable\<^bsub>x\<^esub> expr1" "differentiable\<^bsub>x\<^esub> expr2"
+  shows "\<D>\<^bsub>x\<^esub>\<langle>\<sigma>\<rangle> (expr1 * expr2) = (expr1 * \<D>\<^bsub>x\<^esub>\<langle>\<sigma>\<rangle> expr2 + \<D>\<^bsub>x\<^esub>\<langle>\<sigma>\<rangle> expr1 * expr2)\<^sub>e"
+  using assms by (simp add: expr_defs fun_eq_iff frechet_derivative_mult assms)
+
+lemma lframeD_inner [framed_derivs]:
+  fixes x :: "'c::{real_normed_vector, real_inner} \<Longrightarrow> 'v"
+  assumes "vwb_lens x" "differentiable\<^bsub>x\<^esub> expr1" "differentiable\<^bsub>x\<^esub> expr2"
+  shows "\<D>\<^bsub>x\<^esub>\<langle>\<sigma>\<rangle> (expr1 \<bullet> expr2) = (expr1 \<bullet> \<D>\<^bsub>x\<^esub>\<langle>\<sigma>\<rangle> expr2 + \<D>\<^bsub>x\<^esub>\<langle>\<sigma>\<rangle> expr1 \<bullet> expr2)\<^sub>e"
+  using assms by (simp add: expr_defs fun_eq_iff frechet_derivative_inner)
+
+lemma lframeD_scaleR [framed_derivs]:
+  fixes a :: "'c::{real_normed_vector} \<Longrightarrow> 'v"
+  assumes "vwb_lens x" "differentiable\<^bsub>x\<^esub> expr1" "differentiable\<^bsub>x\<^esub> expr2"
+  shows "\<D>\<^bsub>x\<^esub>\<langle>\<sigma>\<rangle> (expr1 *\<^sub>R expr2) = (expr1 *\<^sub>R \<D>\<^bsub>x\<^esub>\<langle>\<sigma>\<rangle> expr2 + \<D>\<^bsub>x\<^esub>\<langle>\<sigma>\<rangle> expr1 *\<^sub>R expr2)\<^sub>e"
+  using assms by (simp add: expr_defs fun_eq_iff frechet_derivative_scaleR)
+
+lemma lframeD_inverse [framed_derivs]:
+  fixes x :: "'c::real_normed_vector \<Longrightarrow> 's" 
+    and expr :: "'s \<Rightarrow> 'v::real_normed_div_algebra"
+  assumes  "vwb_lens x" "differentiable\<^bsub>x\<^esub> expr" "`expr \<noteq> 0`"
+  shows "\<D>\<^bsub>x\<^esub>\<langle>\<sigma>\<rangle> (inverse expr) = (- (inverse expr * \<D>\<^bsub>x\<^esub>\<langle>\<sigma>\<rangle> expr * inverse expr))\<^sub>e"
+  using assms by (simp add: expr_defs fun_eq_iff frechet_derivative_inverse)
+
+lemma lframeD_divide [framed_derivs]:
+  fixes x :: "'c::real_normed_vector \<Longrightarrow> 's" 
+    and expr1 :: "'s \<Rightarrow> 'v::real_normed_field"
+  assumes  "vwb_lens x" "differentiable\<^bsub>x\<^esub> expr1" "differentiable\<^bsub>x\<^esub> expr2" "`expr2 \<noteq> 0`"
+  shows "\<D>\<^bsub>x\<^esub>\<langle>\<sigma>\<rangle> (expr1 / expr2) = (\<D>\<^bsub>x\<^esub>\<langle>\<sigma>\<rangle> expr1 / expr2 - expr1 * (\<D>\<^bsub>x\<^esub>\<langle>\<sigma>\<rangle> expr2 / expr2\<^sup>2))\<^sub>e"
+  using assms by (simp add: expr_defs fun_eq_iff frechet_derivative_divide)
+
+lemma lframeD_power [framed_derivs]:
+  fixes x :: "'c::ordered_euclidean_space \<Longrightarrow> 's"
+    and expr :: "'s \<Rightarrow> 'v::{ordered_euclidean_space, real_normed_field}"
+  assumes "vwb_lens x" "differentiable\<^bsub>x\<^esub> expr"
+  shows "\<D>\<^bsub>x\<^esub>\<langle>\<sigma>\<rangle> (expr ^ \<guillemotleft>n\<guillemotright>) = (of_nat \<guillemotleft>n\<guillemotright> * \<D>\<^bsub>x\<^esub>\<langle>\<sigma>\<rangle> expr * expr ^ (\<guillemotleft>n\<guillemotright> - 1))\<^sub>e"
+  using assms by (simp add: expr_defs fun_eq_iff frechet_derivative_power)
+
+lemma lframeD_ln [framed_derivs]:
+  fixes x :: "'c::{banach, real_normed_algebra_1} \<Longrightarrow> 's" 
+    and expr :: "'s \<Rightarrow> real"
+  assumes "vwb_lens x" "differentiable\<^bsub>x\<^esub> expr" "`expr > 0`"
+  shows "\<D>\<^bsub>x\<^esub>\<langle>\<sigma>\<rangle> (ln expr) = (\<D>\<^bsub>x\<^esub>\<langle>\<sigma>\<rangle> expr / expr)\<^sub>e"
+  using assms by (simp add: expr_defs frechet_derivative_ln divide_inverse)
+
+lemma lframeD_sin [framed_derivs]:
+  fixes expr :: "'s \<Rightarrow> real"
+  assumes "vwb_lens x" "differentiable\<^bsub>x\<^esub> expr"
+  shows "\<D>\<^bsub>x\<^esub>\<langle>\<sigma>\<rangle> (sin expr) = (\<D>\<^bsub>x\<^esub>\<langle>\<sigma>\<rangle> expr * cos expr)\<^sub>e"
+  using assms by (simp add: expr_defs fun_eq_iff frechet_derivative_sin)
+
+lemma lframeD_cos [framed_derivs]:
+  fixes expr :: "'s \<Rightarrow> real"
+  assumes "vwb_lens x" "differentiable\<^bsub>x\<^esub> expr"
+  shows "\<D>\<^bsub>x\<^esub>\<langle>\<sigma>\<rangle> (cos expr) = (\<D>\<^bsub>x\<^esub>\<langle>\<sigma>\<rangle> expr * - sin expr)\<^sub>e"
+  using assms by (simp add: expr_defs fun_eq_iff frechet_derivative_cos)
+
+declare lens_quotient_plus_den1 [simp]
+declare lens_quotient_plus_den2 [simp]
+
+lemma lframeD_cont_var [framed_derivs]:
+  assumes "vwb_lens X" "x \<subseteq>\<^sub>L X" "bounded_linear (get\<^bsub>x /\<^sub>L X\<^esub>)"
+  shows "\<D>\<^bsub>X\<^esub>\<langle>\<sigma>\<rangle> $x = \<langle>\<sigma>\<rangle>\<^sub>s x"
+  using assms
+  apply (clarsimp simp add: expr_defs lens_quotient_def fun_eq_iff)
+  apply (rename_tac s)
+  apply (subgoal_tac "(\<lambda>c. get\<^bsub>x\<^esub> (put\<^bsub>X\<^esub> s c)) = (\<lambda>c. get\<^bsub>x\<^esub> (create\<^bsub>X\<^esub> c))", simp)
+  apply (metis bounded_linear_imp_has_derivative frechet_derivative_at sublens'_prop2 sublens_implies_sublens' sublens_pres_vwb)
+  apply (metis lens_create_def sublens_obs_get vwb_lens_mwb)
+  done
+
+(* is this a partial derivative? *)
+lemma lframeD_disc_var [framed_derivs]:
+  assumes "vwb_lens y" "x \<bowtie> y"
+  shows "\<D>\<^bsub>y\<^esub>\<langle>\<sigma>\<rangle> $x = (0)\<^sub>e"
+  using assms
+  by (auto simp add: expr_defs lens_quotient_def fun_eq_iff)
+
+
+subsection \<open> framed differential invariants \<close>
+
+thm lframe_subst_def[unfolded lframe_fun_alt] tsubst2vecf_eq lframe_fun_alt
+
+lemma has_vector_derivative_expr:
+  fixes x :: "'c::real_normed_vector \<Longrightarrow> 's"
+    and expr :: "'s \<Rightarrow> 'v::real_normed_vector"
+    and \<sigma> :: "'s \<Rightarrow> 's"
+    and \<phi> :: "real \<Rightarrow> 'c"
+  assumes "vwb_lens x" "differentiable\<^bsub>x\<^esub> expr" 
+    and "(\<phi> has_vector_derivative (\<sigma> \<down>\<^sub>S\<^sub>u\<^sub>b\<^sub>s\<^sub>t\<^bsub>x\<^esub> s) (\<phi> t)) (at t within A)"
+  shows "((expr\<down>\<^sub>F\<^bsub>x\<^esub> s) \<circ> \<phi> has_vector_derivative (\<D>\<^bsub>x\<^esub>\<langle>\<sigma>\<rangle> expr) (put\<^bsub>x\<^esub> s (\<phi> t))) (at t within A)"
+  using assms
+  apply (simp add: lens_defs expr_defs frechet_derivative_works)
+  apply (rule vector_derivative_diff_chain_within)
+   apply blast
+  apply (rule has_derivative_at_withinI)
+  apply (drule_tac x="put\<^bsub>x\<^esub> s (\<phi> t)" in spec)
+  apply (simp)
+  done
+
+lemma lie_diff_inv_on_eq:
+  fixes e :: "'s \<Rightarrow> _::real_inner" and a :: "'c::real_normed_vector \<Longrightarrow> 's"
+  assumes "vwb_lens a" "differentiable\<^sub>e e on a" "`B \<longrightarrow> \<L>\<^bsub>F\<^esub> e on a = 0`"
+  shows "diff_inv_on a (\<lambda> _. F) (B)\<^sub>e ({t. t \<ge> 0})\<^sub>e UNIV 0 (e = 0)\<^sub>e"
+  using assms apply(simp_all add: diff_inv_on_eq ivp_sols_def tsubst2vecf_eq)
+proof(auto simp: lens_defs expr_defs)
+  fix t :: real and X :: "real \<Rightarrow> 'c" and s :: "'s"
+  assume a1:"\<forall>s. (\<lambda>x. e (put\<^bsub>a\<^esub> s x)) differentiable at (get\<^bsub>a\<^esub> s)" and a2: "0 \<le> t" 
+    and a3: "(X has_vderiv_on (\<lambda>x. get\<^bsub>a\<^esub> (F (put\<^bsub>a\<^esub> s (X x))))) (Collect ((\<le>) 0))" 
+    "\<forall>\<tau>. 0 \<le> \<tau> \<and> \<tau> \<le> t \<longrightarrow> B (put\<^bsub>a\<^esub> s (X \<tau>))" and a5: "X 0 = get\<^bsub>a\<^esub> s" and a6: "e s = 0"
+    and a4: "\<forall>s. B s \<longrightarrow> \<partial> (\<lambda>x. e (put\<^bsub>a\<^esub> s x)) (at (get\<^bsub>a\<^esub> s)) (get\<^bsub>a\<^esub> (F s)) = 0"
+  show "(\<lambda>x. e (put\<^bsub>a\<^esub> s x)) (X t) = 0"
+  proof (cases "t = 0")
+    case True
+    then show ?thesis
+      using a5 a6 assms(1) by auto
+  next
+    case False
+    hence t: "t > 0"
+      using a2 by linarith
+    have g: "\<forall>t\<in>{0..t}. B (put\<^bsub>a\<^esub> s (X t))"
+      by (simp add: a3(2))
+    hence d0: "\<forall>t\<in>{0..t}. \<partial> (\<lambda>x. e (put\<^bsub>a\<^esub> s x)) (at (X t)) (get\<^bsub>a\<^esub> (F (put\<^bsub>a\<^esub> s (X t)))) = 0"
+      using a4 by (auto simp add: assms(1))
+    from a1 have dE: "\<forall>\<tau>\<in>{0..t}. ((\<lambda>x. e (put\<^bsub>a\<^esub> s x)) has_derivative \<partial> (\<lambda>x. e (put\<^bsub>a\<^esub> s x)) (at (X \<tau>))) (at (X \<tau>))"
+      by (auto simp add: frechet_derivative_works, drule_tac x="put\<^bsub>a\<^esub> s (X \<tau>)" in spec, simp add: assms)
+    have d1: "\<forall>\<tau>\<in>{0..t}. ((\<lambda>x. e (put\<^bsub>a\<^esub> s x)) \<circ> X has_vector_derivative (\<L>\<^bsub>F\<^esub> e on a) (put\<^bsub>a\<^esub> s (X \<tau>))) (at \<tau> within {0..t})"
+      using a3 apply(clarsimp simp: has_vderiv_on_def)
+      apply (rule derivation_lemma1[OF assms(1,2)], simp add: has_vector_derivative_def)
+      by (rule has_derivative_subset[of _ _ _ "Collect ((\<le>) 0)"], auto)
+    hence d2: "\<forall>\<tau>\<in>{0..t}. ((\<lambda>x. e (put\<^bsub>a\<^esub> s x)) \<circ> X has_vector_derivative 0) (at \<tau> within {0..t})"
+      using a4 g apply(subst (asm) lie_deriv_on_def)
+      by (metis SEXP_def)
+    have c: "continuous_on {0..t} ((\<lambda>x. e (put\<^bsub>a\<^esub> s x)) \<circ> X)"
+      using continuous_on_vector_derivative d2 by fastforce
+    have d3: "(\<And>x. 0 < x \<Longrightarrow> x < t \<Longrightarrow> D ((\<lambda>x. e (put\<^bsub>a\<^esub> s x)) \<circ> X) \<mapsto> (\<lambda>x. 0) at x)"
+      by (metis atLeastAtMost_iff at_within_Icc_at d2 frechet_derivative_at has_derivative_const has_vector_derivative_const has_vector_derivative_def less_eq_real_def)
+    have "\<parallel>((\<lambda>x. e (put\<^bsub>a\<^esub> s x)) \<circ> X) t - ((\<lambda>x. e (put\<^bsub>a\<^esub> s x)) \<circ> X) 0\<parallel> \<le> \<parallel>0\<parallel>"
+      using mvt_general[OF t c d3] by auto
+    hence "((\<lambda>x. e (put\<^bsub>a\<^esub> s x)) \<circ> X) t - ((\<lambda>x. e (put\<^bsub>a\<^esub> s x)) \<circ> X) 0 = 0" by simp
+    thus "(\<lambda>x. e (put\<^bsub>a\<^esub> s x)) (X t) = 0"
+      by (simp add: a6 a5 assms(1))
+  qed
+qed
+
+lemma lie_diff_inv_simple:
+  fixes e :: "'s::real_normed_vector \<Rightarrow> real"
+  assumes "differentiable\<^sub>e e" "`B \<longrightarrow> \<L>\<^bsub>F\<^esub> e = 0`"
+  shows "diff_inv ({t. t \<ge> 0})\<^sub>e UNIV (B)\<^sub>e (\<lambda> _. F) 0 (e = 0)\<^sub>e "
+  apply (simp add: diff_inv_on_id_lens[THEN sym])
+  apply (rule lie_diff_inv_on_eq)
+    apply (simp_all add: assms)
+  done
+
+lemma lie_diff_inv_on_le_less:
+  fixes e :: "'s \<Rightarrow> real" and a :: "'c::real_normed_vector \<Longrightarrow> 's"
+  assumes "vwb_lens a" "differentiable\<^sub>e e on a" "`B \<longrightarrow> \<L>\<^bsub>F\<^esub> e on a \<ge> 0`"
+  shows lie_diff_inv_on_leq: "diff_inv_on a (\<lambda> _. F) (B)\<^sub>e ({t. t \<ge> 0})\<^sub>e UNIV 0 (e \<ge> 0)\<^sub>e"
+    and lie_diff_inv_on_less: "diff_inv_on a (\<lambda> _. F) (B)\<^sub>e ({t. t \<ge> 0})\<^sub>e UNIV 0 (e > 0)\<^sub>e"
+  using assms apply(simp_all add: diff_inv_on_eq ivp_sols_def tsubst2vecf_eq)
+proof(auto simp: lens_defs expr_defs)
+  fix t :: real and X :: "real \<Rightarrow> 'c" and s :: "'s"
+  assume a1:"\<forall>s. (\<lambda>x. e (put\<^bsub>a\<^esub> s x)) differentiable at (get\<^bsub>a\<^esub> s)" and a2: "0 \<le> t" 
+    and a3: "(X has_vderiv_on (\<lambda>x. get\<^bsub>a\<^esub> (F (put\<^bsub>a\<^esub> s (X x))))) (Collect ((\<le>) 0))" 
+    "\<forall>\<tau>. 0 \<le> \<tau> \<and> \<tau> \<le> t \<longrightarrow> B (put\<^bsub>a\<^esub> s (X \<tau>))" and a5: "X 0 = get\<^bsub>a\<^esub> s"
+    and a4: "\<forall>s. B s \<longrightarrow> 0 \<le> \<partial> (\<lambda>x. e (put\<^bsub>a\<^esub> s x)) (at (get\<^bsub>a\<^esub> s)) (get\<^bsub>a\<^esub> (F s))"
+  have g: "\<forall>t\<in>{0..t}. B (put\<^bsub>a\<^esub> s (X t))"
+    by (simp add: a3(2))
+  hence d0: "\<forall>t\<in>{0..t}. 0 \<le> \<partial> (\<lambda>x. e (put\<^bsub>a\<^esub> s x)) (at (X t)) (get\<^bsub>a\<^esub> (F (put\<^bsub>a\<^esub> s (X t))))"
+    using a4 by (auto simp: assms(1))
+  from a1 have dE: "\<forall>\<tau>\<in>{0..t}. ((\<lambda>x. e (put\<^bsub>a\<^esub> s x)) has_derivative \<partial> (\<lambda>x. e (put\<^bsub>a\<^esub> s x)) (at (X \<tau>))) (at (X \<tau>))"
+    by (auto simp add: frechet_derivative_works, drule_tac x="put\<^bsub>a\<^esub> s (X \<tau>)" in spec, simp add: assms)
+  have d1: "\<forall>\<tau>\<in>{0..t}. ((\<lambda>x. e (put\<^bsub>a\<^esub> s x)) \<circ> X has_vector_derivative (\<L>\<^bsub>F\<^esub> e on a) (put\<^bsub>a\<^esub> s (X \<tau>))) (at \<tau> within {0..t})"
+    using a3 apply(clarsimp simp: has_vderiv_on_def)
+    apply (rule derivation_lemma1[OF assms(1,2)], simp add: has_vector_derivative_def)
+    by (rule has_derivative_subset[of _ _ _ "Collect ((\<le>) 0)"], auto)
+  hence "\<forall>\<tau>\<in>{0..t}. ((\<lambda>x. e (put\<^bsub>a\<^esub> s x)) \<circ> X has_derivative (\<lambda>x. x *\<^sub>R (\<L>\<^bsub>F\<^esub> e on a) (put\<^bsub>a\<^esub> s (X \<tau>)))) (at \<tau> within {0..t})"
+    unfolding has_vector_derivative_def by simp
+  hence "\<exists>x\<in>{0..t}. ((\<lambda>x. e (put\<^bsub>a\<^esub> s x)) \<circ> X) t - ((\<lambda>x. e (put\<^bsub>a\<^esub> s x)) \<circ> X) 0 = (t - 0) *\<^sub>R (\<L>\<^bsub>F\<^esub> e on a) (put\<^bsub>a\<^esub> s (X x))"
+    using mvt_very_simple[OF a2, of "(\<lambda>x. e (put\<^bsub>a\<^esub> s x)) \<circ> X" "\<lambda>\<tau> t. t *\<^sub>R (\<L>\<^bsub>F\<^esub> e on a) (put\<^bsub>a\<^esub> s (X \<tau>))"]
+    using atLeastAtMost_iff by blast
+  then obtain \<tau> where final: "0 \<le> \<tau>" "\<tau> \<le> t" 
+    "0 \<le> \<partial> (\<lambda>x. e (put\<^bsub>a\<^esub> s x)) (at (X \<tau>)) (get\<^bsub>a\<^esub> (F (put\<^bsub>a\<^esub> s (X \<tau>))))"
+    "e (put\<^bsub>a\<^esub> s (X t)) - e (put\<^bsub>a\<^esub> s (X 0)) = t * (\<L>\<^bsub>F\<^esub> e on a) (put\<^bsub>a\<^esub> s (X \<tau>))"
+    using lie_deriv_on_def[of F e a] d0 by auto
+  thus "0 \<le> e s \<Longrightarrow> 0 \<le> e (put\<^bsub>a\<^esub> s (X t))"
+    using assms(1) a5 apply(clarsimp simp: lie_deriv_on_def)
+    by (smt split_mult_pos_le)
+  show "0 < e s \<Longrightarrow> 0 < e (put\<^bsub>a\<^esub> s (X t))"
+    using final assms(1) a5 apply(clarsimp simp: lie_deriv_on_def)
+    by (smt split_mult_pos_le)
+qed
+
+lemma lie_deriv_eq_rule:
+  fixes e :: "'s \<Rightarrow> 'a::real_inner" and a :: "'c::real_normed_vector \<Longrightarrow> 's"
+  assumes "vwb_lens a" "differentiable\<^sub>e e on a" "differentiable\<^sub>e f on a"
+  shows lie_deriv_eq: "`B \<longrightarrow> \<L>\<^bsub>F\<^esub> e on a = \<L>\<^bsub>F\<^esub> f on a` 
+  \<Longrightarrow> diff_inv_on a (\<lambda> _. F) (B)\<^sub>e ({t. t \<ge> 0})\<^sub>e UNIV 0 (e = f)\<^sub>e " (is "_ \<Longrightarrow> ?thesis1")
+proof -
+  have "`B \<longrightarrow> \<L>\<^bsub>F\<^esub> e on a = \<L>\<^bsub>F\<^esub> f on a` \<Longrightarrow> diff_inv_on a (\<lambda> _. F) (B)\<^sub>e ({t. t \<ge> 0})\<^sub>e UNIV 0 (e - f = 0)\<^sub>e"
+    by (rule lie_diff_inv_on_eq, simp_all add: lie_deriv closure assms)
+  moreover have "(e - f = 0)\<^sub>e = (e = f)\<^sub>e"
+    by (simp add: expr_defs)
+  ultimately show "`B \<longrightarrow> \<L>\<^bsub>F\<^esub> e on a = \<L>\<^bsub>F\<^esub> f on a` \<Longrightarrow> ?thesis1"
+    by simp
+qed
+
+lemma lie_deriv_le_rule:
+  fixes e :: "'s \<Rightarrow> real" and a :: "'c::real_normed_vector \<Longrightarrow> 's"
+  assumes "vwb_lens a" "differentiable\<^sub>e e on a" "differentiable\<^sub>e f on a"
+  shows lie_deriv_le: "`B \<longrightarrow> \<L>\<^bsub>F\<^esub> f on a \<le> \<L>\<^bsub>F\<^esub> e on a` 
+  \<Longrightarrow> diff_inv_on a (\<lambda> _. F) (B)\<^sub>e ({t. t \<ge> 0})\<^sub>e UNIV 0 (e \<ge> f)\<^sub>e " (is "_ \<Longrightarrow> ?thesis2")
+proof -
+  have "`B \<longrightarrow> \<L>\<^bsub>F\<^esub> f on a \<le> \<L>\<^bsub>F\<^esub> e on a` \<Longrightarrow> diff_inv_on a (\<lambda> _. F) (B)\<^sub>e  ({t. t \<ge> 0})\<^sub>e UNIV 0 (e - f \<ge> 0)\<^sub>e"
+    by (rule lie_diff_inv_on_leq, simp_all add: lie_deriv closure assms)
+  moreover have "(e - f \<ge> 0)\<^sub>e = (e \<ge> f)\<^sub>e"
+    by (simp add: expr_defs)
+  ultimately show "`B \<longrightarrow> \<L>\<^bsub>F\<^esub> f on a \<le> \<L>\<^bsub>F\<^esub> e on a` \<Longrightarrow> ?thesis2"
+    by simp
+qed
+
+lemma lie_deriv_less_rule:
+  fixes e :: "'s \<Rightarrow> real" and a :: "'c::real_normed_vector \<Longrightarrow> 's"
+  assumes "vwb_lens a" "differentiable\<^sub>e e on a" "differentiable\<^sub>e f on a"
+  shows lie_deriv_less: "`B \<longrightarrow> \<L>\<^bsub>F\<^esub> f on a \<le> \<L>\<^bsub>F\<^esub> e on a` \<Longrightarrow> diff_inv_on a (\<lambda> _. F) (B)\<^sub>e ({t. t \<ge> 0})\<^sub>e UNIV 0 (e > f)\<^sub>e " (is "_ \<Longrightarrow> ?thesis2")
+proof -
+  have "`B \<longrightarrow> \<L>\<^bsub>F\<^esub> f on a \<le> \<L>\<^bsub>F\<^esub> e on a` \<Longrightarrow> diff_inv_on a (\<lambda> _. F) (B)\<^sub>e ({t. t \<ge> 0})\<^sub>e UNIV 0 (e - f > 0)\<^sub>e "
+    by (rule lie_diff_inv_on_less, simp_all add: lie_deriv closure assms)
+  moreover have "(e - f \<ge> 0)\<^sub>e = (e \<ge> f)\<^sub>e"
+    by (simp add: expr_defs)
+  ultimately show "`B \<longrightarrow> \<L>\<^bsub>F\<^esub> f on a \<le> \<L>\<^bsub>F\<^esub> e on a` \<Longrightarrow> ?thesis2"
+    by simp
+qed
 
 named_theorems diff_inv_on_intros "intro rules for certifying (localised) differential invariants"
 
